compiler/dsl/coq/ReflexFrontend.v
@@ -12,12 +12,12 @@ Record spec :=
 ; COMPTDEC : forall (x y : COMPT), decide (x = y)
 ; COMPS    : COMPT -> compd
 ; IMSG     : msg PAYD
-; INIT     : init_prog PAYD COMPT COMPS KSTD IMSG IENVD
+; INIT     : init_prog PAYD COMPT COMPS KSTD IENVD
 ; HANDLERS : handlers PAYD COMPT COMPS KSTD
 }.
 
 Definition mk_main (s : spec) :=
-  @main _ (PAYD s) (COMPT s) (COMPTDEC s) (COMPS s) (KSTD s) (IENVD s) (IMSG s) (INIT s) (HANDLERS s).
+  @main _ (PAYD s) (COMPT s) (COMPTDEC s) (COMPS s) (KSTD s) (IENVD s) (INIT s) (HANDLERS s).
 
 Fixpoint mk_vdesc' l : vdesc' (List.length l) :=
   match l with
@@ -45,13 +45,13 @@ Notation " [ x ] " := (cons x nil).
 Notation " [ x ; .. ; y ] " := (cons x .. (cons y nil) ..).
 
 Definition cast_m_expr {NB_MSG} {PAYD : vvdesc NB_MSG} {KSTD envd} {m : msg PAYD} {t p d}
-  (EQ : Build_msg PAYD t p = m) (e : expr PAYD KSTD (Build_msg PAYD t p) envd d)
-  : expr PAYD KSTD m envd d
+  (EQ : Build_msg PAYD t p = m) (e : expr (hdlr_term PAYD KSTD (Build_msg PAYD t p) envd) d)
+  : expr (hdlr_term PAYD KSTD m envd) d
   :=
-  match EQ in _ = _m return expr _ _ _m _ _ with
+  match EQ in _ = _m return expr (hdlr_term _  _ _m _) _ with
   | Logic.eq_refl => e
   end.
 
 Definition mvar {NB_MSG} {PAYD : vvdesc NB_MSG} {KSTD envd} {m : msg PAYD} {t p}
   (EQ : Build_msg PAYD t p = m) i :=
-  cast_m_expr EQ (MVar PAYD KSTD (Build_msg PAYD t p) envd i).
+  cast_m_expr EQ (Term _ (MVar PAYD KSTD (Build_msg PAYD t p) envd i)).
